Powers.dfy
@@ -8,21 +8,23 @@ module Powers
         else b * power(b, e - 1)
     }
 
-    lemma {:induction e} power_base_one_lema(e: nat) 
+    lemma {:induction e} power_base_one_lemma(e: nat) 
         ensures power(1, e) == 1;
     {
         reveal power();
     }
 
-    lemma {:induction e} power_add_one_lema(b:int, e:nat)
+    lemma {:induction e} power_add_one_lemma(b:int, e:nat)
         ensures power(b, e) * b == power(b, e + 1);
     {
         reveal power();
     }
 
-    lemma power_same_exp_lema(a: int, b: int, e: nat)
+    lemma power_same_exp_lemma(a: int, b: int, e: nat)
         ensures power(a, e) * power(b, e) == power(a * b, e);
     {
         assume false;
     }
+
+    lemma power_mod_lemma
 }
