simrsa.dfy
@@ -7,13 +7,13 @@ function method power(b:int, e:nat) : int
     else b * power(b ,e - 1)
 }
 
-lemma {:induction e} exp_one_rule_lema(e: nat)
+lemma {:induction e} exp_one_rule_lemma(e: nat)
     ensures power(1, e) == 1;
 {
     assert true;
 }
 
-lemma {:induction e, e_1} exp_product_lema(b:int, e:nat, e_1:nat, e_2:nat)
+lemma {:induction e, e_1} exp_product_lemma(b:int, e:nat, e_1:nat, e_2:nat)
 	requires e_1 + e_2 == e; 
 	ensures power(b, e) == power(b, e_1) * power(b, e_2)
 {
@@ -25,7 +25,7 @@ lemma {:induction e, e_1} exp_product_lema(b:int, e:nat, e_1:nat, e_2:nat)
 	}
 }
 
-lemma {:induction e, e_2} exp_power_lema_1(b:int, e: nat, e_1:nat, e_2:nat)
+lemma {:induction e, e_2} exp_power_lemma_1(b:int, e: nat, e_1:nat, e_2:nat)
     decreases e, e_2;
     requires e == e_1 * e_2
     ensures power(b, e) == power(power(b, e_1), e_2)
@@ -43,7 +43,7 @@ lemma {:induction e, e_2} exp_power_lema_1(b:int, e: nat, e_1:nat, e_2:nat)
                 power(1, e_2);
                 ==
                 {
-                    exp_one_rule_lema(e_2);
+                    exp_one_rule_lemma(e_2);
                 }
                 1;
             }
@@ -54,17 +54,17 @@ lemma {:induction e, e_2} exp_power_lema_1(b:int, e: nat, e_1:nat, e_2:nat)
                 power(b, e_1 * e_2);
                 ==
                 {
-                    exp_product_lema(b, e_1 * e_2, e_1 * (e_2 - 1), e_1);
+                    exp_product_lemma(b, e_1 * e_2, e_1 * (e_2 - 1), e_1);
                 }
                 power(b, e_1 * (e_2 - 1)) *  power(b, e_1);
                 ==
                 {
-                    exp_power_lema_1(b, e_1 * (e_2 - 1), e_1, e_2 -1);
+                    exp_power_lemma_1(b, e_1 * (e_2 - 1), e_1, e_2 -1);
                 }
                 power(power(b, e_1), e_2 - 1) *  power(b, e_1);
                 ==
                 {
-                    exp_product_lema(power(b, e_1), e_2, e_2 - 1, 1);
+                    exp_product_lemma(power(b, e_1), e_2, e_2 - 1, 1);
                 }
                 power(power(b, e_1), e_2);
             }
@@ -78,13 +78,13 @@ predicate congruent_def(a: int, b: int, n: int)
 }
 
 
-lemma mul_distrubtive_lema(n: int, a: int, b: int, c: int)
+lemma mul_distrubtive_lemma(n: int, a: int, b: int, c: int)
     ensures n * (a + b + c) == n * a + n * b  + n * c;
 {
     assert true;
 }
 
-lemma mod_mul_lema(a_1: int, a_2: int, b_1: int, b_2: int, n: int)
+lemma mod_mul_lemma(a_1: int, a_2: int, b_1: int, b_2: int, n: int)
     requires congruent_def(a_1, b_1, n) && congruent_def(a_2, b_2, n);
     ensures congruent_def(a_1 * a_2, b_1 * b_2, n);
 {
@@ -105,7 +105,7 @@ lemma mod_mul_lema(a_1: int, a_2: int, b_1: int, b_2: int, n: int)
         n * (n * k_1 * k_2) + n * (b_1 * k_2) + n * (k_1 * b_2);
         ==
         {
-            mul_distrubtive_lema(n, n * k_1 * k_2, b_1 * k_2, k_1 * b_2);
+            mul_distrubtive_lemma(n, n * k_1 * k_2, b_1 * k_2, k_1 * b_2);
         }
         n * (n * k_1 * k_2 + b_1 * k_2 + k_1 * b_2);
     }
@@ -114,7 +114,7 @@ lemma mod_mul_lema(a_1: int, a_2: int, b_1: int, b_2: int, n: int)
     assert congruent_def(a_1 * a_2, b_1 * b_2, n);
 }
 
-lemma {:induction e} mod_exp_lema(b: int, e: nat, m: nat)
+lemma {:induction e} mod_exp_lemma(b: int, e: nat, m: nat)
     requires m >= 2;
     ensures power(b, e) % m == (power(b % m , e)) % m
 {
